finished all proof of callback example

demo/ClientServerCspec.v
@@ -170,13 +170,27 @@ Proof.
   eapply preserves_fsim. eapply spec1_ro; eauto.
 Qed.
 
-(* 
-  need a match_state or sound_state relation
-  different function entry pointers need different signatures.
-*)
+
+Definition wt_inv :  (Genv.symtbl * signature) -> state -> Prop := fun _ _ => True.
+
+Lemma spec1_wt : preserves top_spec1 wt_c wt_c wt_inv.
+Proof.
+  intros [se0 sg] se1 Hse Hw. cbn in Hw. subst.
+  split; cbn in *.
+  - intros. inv H0; inv H.
+    + simpl in SET. constructor.
+    + constructor; eauto.
+    + constructor; eauto.
+  - intros. inv H. inv H0. constructor; eauto.
+    constructor. constructor.
+  - intros. inv H0.
+  - intros. inv H0. inv H. constructor; eauto.
+Qed.
+
 Theorem top1_wt : forward_simulation wt_c wt_c top_spec1 top_spec1.
 Proof.
-Admitted.
+  eapply preserves_fsim. eapply spec1_wt; eauto.
+Qed.
 
 
 
